Incorrectness/SPExamples.lean
@@ -1,4 +1,5 @@
 import Incorrectness.SP
+import Incorrectness.While
 
 open Language
 open Incorrectness
